build.sh
@@ -1,3 +1,3 @@
 #todo: clean if makefile exists
 coq_makefile -f _CoqProject -o Makefile
-make
+make -j8
